SELFOUR-1016: fix confused deputy problem when setting priorities

spec/haskell/src/SEL4/API/Invocation.lhs
@@ -60,8 +60,8 @@ The following data type defines the set of possible TCB invocation operations. T
 >             tcThread :: PPtr TCB,
 >             tcThreadCapSlot :: PPtr CTE,
 >             tcNewFaultEP :: Maybe CPtr,
->             tcNewMCPriority :: Maybe Priority,
->             tcNewPriority :: Maybe Priority,
+>             tcNewMCPriority :: Maybe (Priority, PPtr TCB),
+>             tcNewPriority :: Maybe (Priority, PPtr TCB),
 >             tcNewCRoot, tcNewVRoot :: Maybe (Capability, PPtr CTE),
 >             tcNewIPCBuffer :: Maybe (VPtr, Maybe (Capability, PPtr CTE)) }
 >         | NotificationControl {
