spec/abstract/Invocations_A.thy
@@ -51,8 +51,8 @@ datatype tcb_invocation =
   | CopyRegisters machine_word machine_word bool bool bool bool arch_copy_register_sets
   | ThreadControl machine_word cslot_ptr
                   (tc_new_fault_ep: "cap_ref option")
-                  (tc_new_mcpriority: "word8 option")
-                  (tc_new_priority: "word8 option")
+                  (tc_new_mcpriority: "(word8 * obj_ref) option")
+                  (tc_new_priority: "(word8 * obj_ref) option")
                   (tc_new_croot: "(cap * cslot_ptr) option")
                   (tc_new_vroot: "(cap * cslot_ptr) option")
                   (tc_new_buffer: "(vspace_ref * (cap * cslot_ptr) option) option")
