proof/crefine/ARM_HYP/Tcb_C.thy
@@ -582,8 +582,8 @@ lemma invokeTCB_ThreadControl_ccorres:
    (UNIV \<inter> {s. target_' s = tcb_ptr_to_ctcb_ptr target}
          \<inter> {s. (cRoot \<noteq> None \<or> buf \<noteq> None) \<longrightarrow> slot_' s = cte_Ptr slot}
          \<inter> {s. faultep_' s = option_to_0 faultep}
-         \<inter> {s. mcp_' s = case_option 0 ucast mcp}
-         \<inter> {s. priority_' s = case_option 0 ucast priority}
+         \<inter> {s. mcp_' s = case_option 0 (ucast o fst) mcp}
+         \<inter> {s. priority_' s = case_option 0 (ucast o fst) priority}
          \<inter> {s. case cRoot of None \<Rightarrow> True | Some (cRootCap, cRootSlot) \<Rightarrow> ccap_relation cRootCap (cRoot_newCap_' s)}
          \<inter> {s. cRoot_srcSlot_' s = cte_Ptr (option_to_0 (option_map snd cRoot))}
          \<inter> {s. case vRoot of None \<Rightarrow> True | Some (vRootCap, vRootSlot) \<Rightarrow> ccap_relation vRootCap (vRoot_newCap_' s)}
@@ -2803,15 +2803,6 @@ lemma from_bool_all_helper:
       = ((\<exists>bool. from_bool bool = val) \<longrightarrow> P (val \<noteq> 0))"
   by (auto simp: from_bool_0)
 
-lemma thread_control_update_all_or:
-  "thread_control_update_all
-     = thread_control_update_mcp
-        || thread_control_update_priority
-        || thread_control_update_ipc_buffer
-        || thread_control_update_space"
-  apply (simp add: thread_control_flag_defs)
-  done
-
 lemma getSyscallArg_ccorres_foo':
   "ccorres (\<lambda>a rv. rv = ucast (args ! n)) (\<lambda>x. ucast (ret__unsigned_long_' x))
          (sysargs_rel args buffer and sysargs_rel_n args buffer n)
@@ -2841,24 +2832,16 @@ lemma tcb_at_capTCBPtr_CL:
   apply (frule ctcb_ptr_to_tcb_ptr_mask[OF tcb_aligned'], simp)
   done
 
-lemma prioPropsFromWord_spec:
-  "\<forall>s. \<Gamma> \<turnstile> \<lbrace>s. True\<rbrace> Call prioPropsFromWord_'proc
-  \<lbrace> seL4_PrioProps_lift \<acute>ret__struct_seL4_PrioProps_C =
-      \<lparr>  mcp_CL =  (\<^bsup>s\<^esup>w >> 8) && mask 8,
-        prio_CL = (\<^bsup>s\<^esup>w) && mask 8 \<rparr>  \<rbrace>"
-  by vcg (simp add: seL4_PrioProps_lift_def mask_def)
-
 lemma checkPrio_ccorres:
   "ccorres (syscall_error_rel \<currency> dc) (liftxf errstate id (K ()) ret__unsigned_long_')
-      \<top>
-      (UNIV \<inter> {s. prio_' s = prio}) []
-      (checkPrio prio)
+      (tcb_at' auth)
+      (UNIV \<inter> {s. prio_' s = prio} \<inter> {s. auth_' s = tcb_ptr_to_ctcb_ptr auth}) []
+      (checkPrio prio auth)
       (Call checkPrio_'proc)"
-  apply (cinit lift: prio_')
+  apply (cinit lift: prio_' auth_')
    apply (clarsimp simp: liftE_bindE)
-   apply (rule ccorres_pre_getCurThread)
    apply (rule ccorres_split_nothrow_novcg[where r'="\<lambda>rv rv'. rv' = ucast rv" and xf'=mcp_'])
-       apply (rule_tac P="\<lambda>s. ct = ksCurThread s" in threadGet_vcg_corres_P)
+       apply (rule threadGet_vcg_corres)
        apply (rule allI, rule conseqPre, vcg)
        apply (clarsimp simp: rf_sr_ksCurThread obj_at'_def projectKOs
                              typ_heap_simps' ctcb_relation_def)
@@ -2980,335 +2963,286 @@ lemma decodeTCBConfigure_ccorres:
           ctac add: getSyscallArg_ccorres_foo[where args=args and n=0 and buffer=buffer])
      apply (rule ccorres_add_return,
             ctac add: getSyscallArg_ccorres_foo'[where args=args and n=1 and buffer=buffer])
-       apply csymbr
        apply (rule ccorres_add_return,
               ctac add: getSyscallArg_ccorres_foo[where args=args and n=2 and buffer=buffer])
          apply (rule ccorres_add_return,
                 ctac add: getSyscallArg_ccorres_foo[where args=args and n=3 and buffer=buffer])
-           apply (rule ccorres_add_return,
-                  ctac add: getSyscallArg_ccorres_foo[where args=args and n=4 and buffer=buffer])
+           apply csymbr
+           apply (rule getSlotCap_ccorres_fudge_n[where vals=extraCaps and n=0])
+           apply (rule ccorres_move_c_guard_cte)
+           apply ctac
+             apply (rule ccorres_assert2)
              apply csymbr
-             apply (rule getSlotCap_ccorres_fudge_n[where vals=extraCaps and n=0])
              apply (rule ccorres_move_c_guard_cte)
+             apply (rule getSlotCap_ccorres_fudge_n[where vals=extraCaps and n=1])
              apply ctac
                apply (rule ccorres_assert2)
                apply csymbr
+               apply (rule getSlotCap_ccorres_fudge_n[where vals=extraCaps and n=2])
                apply (rule ccorres_move_c_guard_cte)
-               apply (rule getSlotCap_ccorres_fudge_n[where vals=extraCaps and n=1])
                apply ctac
                  apply (rule ccorres_assert2)
-                 apply csymbr
-                 apply (rule getSlotCap_ccorres_fudge_n[where vals=extraCaps and n=2])
-                 apply (rule ccorres_move_c_guard_cte)
-                 apply ctac
-                   apply (rule ccorres_assert2)
-                   apply csymbr
-                   apply csymbr
-                   apply (simp add: decodeSetPriority_def decodeSetMCPriority_def priorityBits_def
-                                    bindE_assoc invocationCatch_use_injection_handler
-                                    injection_bindE[OF refl refl] injection_handler_returnOk
-                               del: Collect_const)
-                   apply (rule ccorres_split_nothrowE)
-                        apply (ctac add: ccorres_injection_handler_csum1[OF checkPrio_ccorres])
-                       apply ceqv
-                      apply ccorres_rewrite
-                      apply (rule ccorres_split_nothrowE)
-                           apply (ctac add: ccorres_injection_handler_csum1[OF checkPrio_ccorres])
-                          apply ceqv
-                         apply ccorres_rewrite
-                         apply (simp add: decodeSetIPCBuffer_def split_def
-                                          injection_handler_If injection_handler_returnOk
-                                          injection_bindE [OF refl refl] bindE_assoc
-                                     del: Collect_const cong: if_cong)
-                         apply (rule_tac xf'="\<lambda>s. (bufferCap_' s, bufferSlot_' s)"
-                                      and r'="\<lambda>v (cp', sl'). case v of None \<Rightarrow> args ! 4 = 0 \<and> sl' = cte_Ptr 0
-                                                                     | Some (cp, sl) \<Rightarrow> ccap_relation cp cp'
-                                                                                        \<and> args ! 4 \<noteq> 0
-                                                                                        \<and> sl' = cte_Ptr sl"
-                                  in ccorres_splitE)
-                             apply (rule ccorres_cond2[where R=\<top>])
-                               apply (clarsimp simp add: Collect_const_mem numeral_eqs)
-                              apply (rule_tac P="\<lambda>s. args ! 4 = 0" in ccorres_from_vcg[where P'=UNIV])
-                              apply (rule allI, rule conseqPre, vcg)
-                              apply (clarsimp simp: returnOk_def return_def)
-                             apply (rule ccorres_rhs_assoc)+
-                             apply (rule ccorres_split_nothrowE)
-                                  apply (simp add: numeral_eqs)
-                                  apply (ctac add: ccorres_injection_handler_csum1[OF deriveCap_ccorres])
-                                 apply ceqv
-                                apply simp
-                                apply csymbr
-                                apply (rule ccorres_split_nothrowE)
-                                     apply (ctac add: ccorres_injection_handler_csum1[OF checkValidIPCBuffer_ccorres])
-                                    apply ceqv
-                                   apply (match premises in "ccap_relation _ (deriveCap_ret_C.cap_C ccap)" for ccap
-                                            \<Rightarrow> \<open>rule ccorres_from_vcg
-                                                       [where P'="{s. bufferCap_' s = (deriveCap_ret_C.cap_C ccap)
-                                                                      \<and> bufferSlot_' s = cte_Ptr (snd (extraCaps ! 2))}"
-                                                          and P="\<lambda>s. args ! 4 \<noteq> 0"]\<close>)
-                                   apply (rule allI, rule conseqPre, vcg)
-                                   apply (clarsimp simp: returnOk_def return_def numeral_eqs)
-                                  apply (rule_tac P'="{s. err' = errstate s}"
-                                           in ccorres_from_vcg_throws[where P=\<top>])
-                                  apply (rule allI, rule conseqPre, vcg)
-                                  apply (clarsimp simp: throwError_def return_def
-                                                        syscall_error_rel_def
-                                                        intr_and_se_rel_def)
-                                 apply wp
-                                apply simp
-                                apply (vcg exspec=checkValidIPCBuffer_modifies)
-                               apply simp
-                               apply (rule_tac P'="{s. err' = errstate s}"
-                                        in  ccorres_from_vcg_split_throws[where P=\<top>])
-                                apply vcg
-                               apply (rule conseqPre, vcg)
-                               apply (clarsimp simp: throwError_def return_def
-                                                     intr_and_se_rel_def syscall_error_rel_def)
-                              apply simp
-                              apply (wp injection_wp_E [OF refl])
-                             apply (simp add: all_ex_eq_helper Collect_const_mem numeral_eqs)
-                             apply (vcg exspec=deriveCap_modifies)
-                            apply (rule ceqv_tuple2, ceqv, ceqv)
-                           apply (rename_tac rv'dc)
-                           apply (rule_tac P="P (fst rv'dc) (snd rv'dc)"
-                                       and P'="P' (fst rv'dc) (snd rv'dc)"
-                                    for P P' in ccorres_inst)
-                           apply (clarsimp simp: tcb_cnode_index_defs
-                                                 [THEN ptr_add_assertion_positive
-                                                       [OF ptr_add_assertion_positive_helper]]
-                                           simp del: Collect_const)
-                           apply csymbr
-                           apply (rule ccorres_move_array_assertion_tcb_ctes ccorres_Guard_Seq)+
-                           apply (simp add: decodeSetSpace_def injection_bindE[OF refl] split_def
-                                       del: Collect_const)
-                           apply (simp add: injection_liftE[OF refl] bindE_assoc
-                                            liftM_def getThreadCSpaceRoot
-                                            getThreadVSpaceRoot del: Collect_const)
-                           apply (simp add: liftE_bindE del: Collect_const)
-                           apply (rule ccorres_rhs_assoc)+
-                           apply (ctac add: slotCapLongRunningDelete_ccorres)
-                             apply (rule ccorres_move_array_assertion_tcb_ctes)
-                             apply (simp del: Collect_const)
-                             apply csymbr
-                             apply (clarsimp simp add: if_1_0_0 from_bool_0
-                                             simp del: Collect_const)
-                             apply (rule ccorres_Cond_rhs_Seq)
-                              apply (rule ccorres_symb_exec_l3
-                                          [OF _ _ _ empty_fail_slotCapLongRunningDelete])
-                                apply (simp add: unlessE_def injection_handler_throwError
-                                           cong: StateSpace.state.fold_congs globals.fold_congs)
-                                apply (rule ccorres_cond_true_seq)
-                                apply (rule syscall_error_throwError_ccorres_n)
-                                apply (simp add: syscall_error_to_H_cases)
-                               apply wp+
-                             apply (rule ccorres_rhs_assoc)+
-                             apply csymbr
-                             apply (simp del: Collect_const)
-                             apply (rule ccorres_move_array_assertion_tcb_ctes ccorres_Guard_Seq
-                                         ccorres_rhs_assoc)+
-                             apply (ctac add: slotCapLongRunningDelete_ccorres)
-                               apply (rule ccorres_move_array_assertion_tcb_ctes)
-                               apply (simp del: Collect_const)
-                               apply csymbr
-                               apply (clarsimp simp add: if_1_0_0 from_bool_0
-                                               simp del: Collect_const)
-                               apply (rule ccorres_Cond_rhs_Seq)
-                                apply (simp add: unlessE_def injection_handler_throwError
-                                           cong: StateSpace.state.fold_congs globals.fold_congs)
-                                apply (rule syscall_error_throwError_ccorres_n)
-                                apply (simp add: syscall_error_to_H_cases)
-                               apply (simp add: unlessE_def injection_handler_returnOk
-                                           del: Collect_const)
-                               apply (rule ccorres_add_return,
-                                      rule_tac r'="\<lambda>rv rv'. ccap_relation
-                                                              (if args ! 2 = 0
-                                                                 then fst (hd extraCaps)
-                                                                 else updateCapData False (args ! 2) (fst (hd extraCaps))) rv'"
-                                          and xf'="cRootCap_'"
-                                          in ccorres_split_nothrow)
-                                   apply (rule_tac P'="{s. cRootCap = cRootCap_' s}"
-                                            in ccorres_from_vcg[where P=\<top>])
-                                   apply (rule allI, rule conseqPre, vcg)
-                                   apply (subgoal_tac "extraCaps \<noteq> []")
-                                    apply (clarsimp simp: returnOk_def return_def hd_conv_nth false_def)
-                                    apply fastforce
-                                   apply clarsimp
-                                  apply ceqv
-                                 apply (ctac add: ccorres_injection_handler_csum1
-                                                    [OF deriveCap_ccorres])
-                                    apply (simp add: Collect_False del: Collect_const)
-                                    apply (csymbr, csymbr)
-                                    apply (simp add: cap_get_tag_isCap cnode_cap_case_if
-                                                del: Collect_const)
-                                    apply (rule ccorres_Cond_rhs_Seq)
-                                     apply (simp add: injection_handler_throwError
-                                                cong: StateSpace.state.fold_congs globals.fold_congs)
-                                     apply (rule syscall_error_throwError_ccorres_n)
-                                     apply (simp add: syscall_error_to_H_cases)
-                                    apply (simp add: injection_handler_returnOk del: Collect_const)
-                                    apply (rule ccorres_add_return,
-                                           rule_tac r'="\<lambda>rv rv'. ccap_relation
-                                                                   (if args ! 3 = 0
-                                                                      then fst (extraCaps ! Suc 0)
-                                                                      else updateCapData False (args ! 3) (fst (extraCaps ! Suc 0))) rv'"
-                                               and xf'="vRootCap_'"
-                                               in ccorres_split_nothrow)
-                                        apply (rule_tac P'="{s. vRootCap = vRootCap_' s}"
-                                                 in ccorres_from_vcg[where P=\<top>])
-                                        apply (rule allI, rule conseqPre, vcg)
-                                        apply (clarsimp simp: returnOk_def return_def
-                                                              hd_drop_conv_nth2 false_def)
-                                        apply fastforce
-                                       apply ceqv
-                                      apply (ctac add: ccorres_injection_handler_csum1
-                                                         [OF deriveCap_ccorres])
-                                         apply (simp add: Collect_False del: Collect_const)
-                                         apply csymbr
-                                         apply csymbr
-                                         apply (simp add: from_bool_0 isValidVTableRoot_conv del: Collect_const)
-                                         apply (rule ccorres_Cond_rhs_Seq)
-                                          apply (simp add: injection_handler_throwError
-                                                     cong: StateSpace.state.fold_congs globals.fold_congs)
-                                          apply (rule syscall_error_throwError_ccorres_n)
-                                          apply (simp add: syscall_error_to_H_cases)
-                                         apply (simp add: injection_handler_returnOk ccorres_invocationCatch_Inr
-                                                          performInvocation_def)
-                                         apply (ctac add: setThreadState_ccorres)
-                                           apply csymbr
-                                           apply (ctac(no_vcg) add: invokeTCB_ThreadControl_ccorres)
-                                             apply (simp, rule ccorres_alternative2)
-                                             apply (rule ccorres_return_CE, simp+)
-                                            apply (rule ccorres_return_C_errorE, simp+)[1]
-                                           apply wp
-                                          apply (simp add: o_def)
-                                          apply (wp sts_invs_minor' hoare_case_option_wp)
-                                         apply (simp add: Collect_const_mem cintr_def intr_and_se_rel_def
-                                                          exception_defs
-                                                    cong: option.case_cong)
-                                         apply (vcg exspec=setThreadState_modifies)
-                                        apply simp
-                                        apply (rule ccorres_split_throws, rule ccorres_return_C_errorE, simp+)
-                                        apply vcg
-                                       apply simp
-                                       apply (wp injection_wp_E[OF refl] hoare_drop_imps)
-                                      apply (vcg exspec=deriveCap_modifies)
-                                     apply (simp add: pred_conj_def cong: if_cong)
-                                     apply wp
-                                    apply (simp add: Collect_const_mem)
-                                    apply (vcg)
-                                   apply simp
-                                   apply (rule ccorres_split_throws, rule ccorres_return_C_errorE, simp+)
-                                   apply vcg
-                                  apply (simp cong: if_cong)
-                                  apply (wp injection_wp_E[OF refl] hoare_drop_imps)
-                                 apply (simp add: Collect_const_mem intr_and_se_rel_def
-                                                  syscall_error_rel_def exception_defs
-                                            cong: option.case_cong sum.case_cong)
-                                 apply (simp add: all_ex_eq_helper numeral_eqs)
-                                 apply (vcg exspec=deriveCap_modifies)
-                                apply (simp cong: if_cong)
-                                apply wp
-                               apply (simp add: Collect_const_mem del: Collect_const)
-                               apply vcg
-                              apply (simp cong: if_cong)
-                              apply (wp | wp_once hoare_drop_imps)+
-                             apply (simp add: Collect_const_mem all_ex_eq_helper
-                                        cong: option.case_cong)
-                             apply (vcg exspec=slotCapLongRunningDelete_modifies)
-                            apply (simp cong: if_cong)
-                            apply (wp | wp_once hoare_drop_imps)+
-                           apply (simp add: Collect_const_mem)
-                           apply (vcg exspec=slotCapLongRunningDelete_modifies)
-                          apply (simp add: pred_conj_def cong: if_cong)
-                          apply (wp injection_wp_E[OF refl] checkValidIPCBuffer_ArchObject_wp)
-                          apply simp
-                          apply (wp | wp_once hoare_drop_imps)+
-                         apply (simp add: Collect_const_mem all_ex_eq_helper)
-                         apply (rule_tac P="{s. cRootCap_' s = cRootCap \<and> vRootCap_' s = vRootCap
-                                                \<and> bufferAddr_' s = args ! 4
-                                                \<and> ccap_relation cp cap' \<and> isThreadCap cp
-                                                \<and> is_aligned (capTCBPtr cp) tcbBlockSizeBits
-                                                \<and> ksCurThread_' (globals s) = tcb_ptr_to_ctcb_ptr thread}"
-                                  in conseqPre)
-                          apply (simp add: cong: option.case_cong)
-                          apply (vcg exspec=deriveCap_modifies exspec=checkValidIPCBuffer_modifies)
-                         apply (clarsimp simp: excaps_map_def Collect_const_mem ccHoarePost_def
-                                               numeral_eqs
-                                         cong: option.case_cong)
-                         apply (frule interpret_excaps_eq[rule_format, where n=0], clarsimp)
-                         apply (frule interpret_excaps_eq[rule_format, where n=1], clarsimp)
-                         apply (frule interpret_excaps_eq[rule_format, where n=2], clarsimp)
-                         apply (clarsimp simp: mask_def[where n=4] ccap_rights_relation_def
-                                               rightsFromWord_wordFromRights capTCBPtr_eq
-                                               ptr_val_tcb_ptr_mask2[unfolded mask_def objBits_defs, simplified]
-                                               tcb_cnode_index_defs size_of_def
-                                               option_to_0_def rf_sr_ksCurThread
-                                               StrictC'_thread_state_defs mask_eq_iff_w2p word_size
-                                               thread_control_update_all_or
-                                               from_bool_all_helper all_ex_eq_helper
-                                               ucast_ucast_mask objBits_defs)
-                         apply (subgoal_tac "args \<noteq> [] \<and> extraCaps \<noteq> []")
-                          apply (simp add: word_sle_def cap_get_tag_isCap numeral_eqs
-                                           hd_conv_nth hd_drop_conv_nth2 ucast_ucast_mask8
-                                           word_FF_is_mask split_def
-                                           thread_control_update_priority_def
-                                           thread_control_update_mcp_def
-                                           thread_control_update_space_def
-                                           thread_control_update_ipc_buffer_def)
-                          apply (auto split: option.split elim!: inl_inrE)[1]
-                          apply fastforce+
+                 apply (simp add: decodeSetIPCBuffer_def split_def
+                                  bindE_assoc invocationCatch_use_injection_handler
+                                  injection_bindE[OF refl refl] injection_handler_returnOk
+                                  injection_handler_If
+                             del: Collect_const cong: if_cong)
+                 apply (rule_tac xf'="\<lambda>s. (bufferCap_' s, bufferSlot_' s)" and
+                                 r'="\<lambda>v (cp', sl'). case v of None \<Rightarrow> args ! 3 = 0 \<and> sl' = cte_Ptr 0
+                                                            | Some (cp, sl) \<Rightarrow> ccap_relation cp cp'
+                                                                               \<and> args ! 3 \<noteq> 0
+                                                                               \<and> sl' = cte_Ptr sl"
+                                 in ccorres_splitE)
+                     apply (rule ccorres_cond2[where R=\<top>])
+                       apply (clarsimp simp add: Collect_const_mem numeral_eqs)
+                      apply (rule_tac P="\<lambda>s. args ! 3 = 0" in ccorres_from_vcg[where P'=UNIV])
+                      apply (rule allI, rule conseqPre, vcg)
+                      apply (clarsimp simp: returnOk_def return_def)
+                     apply (rule ccorres_rhs_assoc)+
+                     apply (rule ccorres_split_nothrowE)
+                          apply (simp add: numeral_eqs)
+                          apply (ctac add: ccorres_injection_handler_csum1[OF deriveCap_ccorres])
+                         apply ceqv
                         apply simp
-                        apply (rule_tac P'="{s. err' = errstate s}"
-                                 in  ccorres_from_vcg_split_throws[where P=\<top>])
-                         apply vcg
-                        apply (rule conseqPre, vcg)
-                        apply (clarsimp simp: throwError_def return_def
-                                              intr_and_se_rel_def syscall_error_rel_def)
-                       apply (wp injection_wp_E[OF refl], clarsimp, rule checkPrio_wp)[1]
+                        apply (clarsimp simp: numeral_eqs)
+                        apply csymbr
+                        apply (rule ccorres_split_nothrowE)
+                             apply (ctac add: ccorres_injection_handler_csum1[OF checkValidIPCBuffer_ccorres])
+                            apply ceqv
+                           apply (match premises in "ccap_relation _ (deriveCap_ret_C.cap_C ccap)" for ccap
+                                    \<Rightarrow> \<open>rule ccorres_from_vcg
+                                          [where P'="{s. bufferCap_' s = (deriveCap_ret_C.cap_C ccap)
+                                                         \<and> bufferSlot_' s = cte_Ptr (snd (extraCaps ! 2))}"
+                                             and P="\<lambda>s. args ! 3 \<noteq> 0"]\<close>)
+                           apply (rule allI, rule conseqPre, vcg)
+                           apply (clarsimp simp: returnOk_def return_def numeral_eqs)
+                          apply (rule_tac P'="{s. err' = errstate s}"
+                                          in ccorres_from_vcg_throws[where P=\<top>])
+                          apply (rule allI, rule conseqPre, vcg)
+                          apply (clarsimp simp: throwError_def return_def
+                                                syscall_error_rel_def
+                                                intr_and_se_rel_def)
+                         apply wp
+                        apply simp
+                        apply (vcg exspec=checkValidIPCBuffer_modifies)
+                       apply simp
+                       apply (rule_tac P'="{s. err' = errstate s}"
+                                       in  ccorres_from_vcg_split_throws[where P=\<top>])
+                        apply vcg
+                       apply (rule conseqPre, vcg)
+                       apply (clarsimp simp: throwError_def return_def
+                                             intr_and_se_rel_def syscall_error_rel_def)
                       apply simp
-                      apply vcg
-                     apply simp
-                     apply (rule_tac P'="{s. err' = errstate s}"
-                              in  ccorres_from_vcg_split_throws[where P=\<top>])
-                      apply vcg
-                     apply (rule conseqPre, vcg)
-                     apply (clarsimp simp: throwError_def return_def
-                                           intr_and_se_rel_def syscall_error_rel_def)
-                    apply (wp injection_wp_E[OF refl], clarsimp, rule checkPrio_wp)[1]
-                   apply clarsimp
-                   apply vcg
-                  apply clarsimp
-                  apply (strengthen if_n_updateCapData_valid_strg)
+                      apply (wp injection_wp_E [OF refl])
+                     apply (simp add: all_ex_eq_helper Collect_const_mem numeral_eqs)
+                     apply (vcg exspec=deriveCap_modifies)
+                    apply (rule ceqv_tuple2, ceqv, ceqv)
+                   apply (rename_tac rv'dc)
+                   apply (rule_tac P="P (fst rv'dc) (snd rv'dc)"
+                               and P'="P' (fst rv'dc) (snd rv'dc)"
+                               for P P' in ccorres_inst)
+                   apply (clarsimp simp: tcb_cnode_index_defs
+                                           [THEN ptr_add_assertion_positive
+                                             [OF ptr_add_assertion_positive_helper]]
+                                   simp del: Collect_const)
+                   apply csymbr
+                   apply (rule ccorres_move_array_assertion_tcb_ctes ccorres_Guard_Seq)+
+                   apply (simp add: decodeSetSpace_def injection_bindE[OF refl] split_def
+                               del: Collect_const)
+                   apply (simp add: injection_liftE[OF refl] bindE_assoc
+                                    liftM_def getThreadCSpaceRoot
+                                    getThreadVSpaceRoot del: Collect_const)
+                   apply (simp add: liftE_bindE del: Collect_const)
+                   apply (rule ccorres_rhs_assoc)+
+                   apply (ctac add: slotCapLongRunningDelete_ccorres)
+                     apply (rule ccorres_move_array_assertion_tcb_ctes)
+                     apply (simp del: Collect_const)
+                     apply csymbr
+                     apply (clarsimp simp add: if_1_0_0 from_bool_0
+                                     simp del: Collect_const)
+                     apply (rule ccorres_Cond_rhs_Seq)
+                      apply (rule ccorres_symb_exec_l3
+                                    [OF _ _ _ empty_fail_slotCapLongRunningDelete])
+                        apply (simp add: unlessE_def injection_handler_throwError
+                                    cong: StateSpace.state.fold_congs globals.fold_congs)
+                        apply (rule ccorres_cond_true_seq)
+                        apply (rule syscall_error_throwError_ccorres_n)
+                        apply (simp add: syscall_error_to_H_cases)
+                       apply wp+
+                     apply (rule ccorres_rhs_assoc)+
+                     apply csymbr
+                     apply (simp del: Collect_const)
+                     apply (rule ccorres_move_array_assertion_tcb_ctes ccorres_Guard_Seq
+                                 ccorres_rhs_assoc)+
+                     apply (ctac add: slotCapLongRunningDelete_ccorres)
+                       apply (rule ccorres_move_array_assertion_tcb_ctes)
+                       apply (simp del: Collect_const)
+                       apply csymbr
+                       apply (clarsimp simp add: if_1_0_0 from_bool_0
+                                       simp del: Collect_const)
+                       apply (rule ccorres_Cond_rhs_Seq)
+                        apply (simp add: unlessE_def injection_handler_throwError
+                                    cong: StateSpace.state.fold_congs globals.fold_congs)
+                        apply (rule syscall_error_throwError_ccorres_n)
+                        apply (simp add: syscall_error_to_H_cases)
+                       apply (simp add: unlessE_def injection_handler_returnOk
+                                   del: Collect_const)
+                       apply (rule ccorres_add_return,
+                              rule_tac r'="\<lambda>rv rv'. ccap_relation
+                                                      (if args ! 1 = 0
+                                                       then fst (hd extraCaps)
+                                                       else updateCapData False (args ! 1) (fst (hd extraCaps))) rv'"
+                                   and xf'="cRootCap_'"
+                                   in ccorres_split_nothrow)
+                           apply (rule_tac P'="{s. cRootCap = cRootCap_' s}"
+                                          in ccorres_from_vcg[where P=\<top>])
+                           apply (rule allI, rule conseqPre, vcg)
+                           apply (subgoal_tac "extraCaps \<noteq> []")
+                            apply (clarsimp simp: returnOk_def return_def hd_conv_nth false_def)
+                            apply fastforce
+                           apply clarsimp
+                          apply ceqv
+                         apply (ctac add: ccorres_injection_handler_csum1
+                                            [OF deriveCap_ccorres])
+                            apply (simp add: Collect_False del: Collect_const)
+                            apply (csymbr, csymbr)
+                            apply (simp add: cap_get_tag_isCap cnode_cap_case_if
+                                        del: Collect_const)
+                            apply (rule ccorres_Cond_rhs_Seq)
+                             apply (simp add: injection_handler_throwError
+                                         cong: StateSpace.state.fold_congs globals.fold_congs)
+                             apply (rule syscall_error_throwError_ccorres_n)
+                             apply (simp add: syscall_error_to_H_cases)
+                            apply (simp add: injection_handler_returnOk del: Collect_const)
+                            apply (rule ccorres_add_return,
+                                   rule_tac r'="\<lambda>rv rv'. ccap_relation
+                                                           (if args ! 2 = 0
+                                                            then fst (extraCaps ! Suc 0)
+                                                            else updateCapData False (args ! 2) (fst (extraCaps ! Suc 0))) rv'"
+                                        and xf'="vRootCap_'"
+                                        in ccorres_split_nothrow)
+                                apply (rule_tac P'="{s. vRootCap = vRootCap_' s}"
+                                                in ccorres_from_vcg[where P=\<top>])
+                                apply (rule allI, rule conseqPre, vcg)
+                                apply (clarsimp simp: returnOk_def return_def
+                                                      hd_drop_conv_nth2 false_def)
+                                apply fastforce
+                               apply ceqv
+                              apply (ctac add: ccorres_injection_handler_csum1
+                                                 [OF deriveCap_ccorres])
+                                 apply (simp add: Collect_False del: Collect_const)
+                                 apply csymbr
+                                 apply csymbr
+                                 apply (simp add: from_bool_0 isValidVTableRoot_conv del: Collect_const)
+                                 apply (rule ccorres_Cond_rhs_Seq)
+                                  apply (simp add: injection_handler_throwError
+                                              cong: StateSpace.state.fold_congs globals.fold_congs)
+                                  apply (rule syscall_error_throwError_ccorres_n)
+                                  apply (simp add: syscall_error_to_H_cases)
+                                 apply (simp add: injection_handler_returnOk ccorres_invocationCatch_Inr
+                                                  performInvocation_def)
+                                 apply (ctac add: setThreadState_ccorres)
+                                   apply csymbr
+                                   apply (ctac(no_vcg) add: invokeTCB_ThreadControl_ccorres)
+                                     apply (simp, rule ccorres_alternative2)
+                                     apply (rule ccorres_return_CE, simp+)
+                                    apply (rule ccorres_return_C_errorE, simp+)[1]
+                                   apply wp
+                                  apply (simp add: o_def)
+                                  apply (wp sts_invs_minor' hoare_case_option_wp)
+                                 apply (simp add: Collect_const_mem cintr_def intr_and_se_rel_def
+                                                  exception_defs
+                                            cong: option.case_cong)
+                                 apply (vcg exspec=setThreadState_modifies)
+                                apply simp
+                                apply (rule ccorres_split_throws, rule ccorres_return_C_errorE, simp+)
+                                apply vcg
+                               apply simp
+                               apply (wp injection_wp_E[OF refl] hoare_drop_imps)
+                              apply (vcg exspec=deriveCap_modifies)
+                             apply (simp add: pred_conj_def cong: if_cong)
+                             apply wp
+                            apply (simp add: Collect_const_mem)
+                            apply (vcg)
+                           apply simp
+                           apply (rule ccorres_split_throws, rule ccorres_return_C_errorE, simp+)
+                           apply vcg
+                          apply (simp cong: if_cong)
+                          apply (wp injection_wp_E[OF refl] hoare_drop_imps)
+                         apply (simp add: Collect_const_mem intr_and_se_rel_def
+                                          syscall_error_rel_def exception_defs
+                                    cong: option.case_cong sum.case_cong)
+                         apply (simp add: all_ex_eq_helper numeral_eqs)
+                         apply (vcg exspec=deriveCap_modifies)
+                        apply (simp cong: if_cong)
+                        apply wp
+                       apply (simp add: Collect_const_mem del: Collect_const)
+                       apply vcg
+                      apply (simp cong: if_cong)
+                      apply (wp | wp_once hoare_drop_imps)+
+                     apply (simp add: Collect_const_mem all_ex_eq_helper
+                                cong: option.case_cong)
+                     apply (vcg exspec=slotCapLongRunningDelete_modifies)
+                    apply (simp cong: if_cong)
+                    apply (wp | wp_once hoare_drop_imps)+
+                   apply (simp add: Collect_const_mem)
+                   apply (vcg exspec=slotCapLongRunningDelete_modifies)
+                  apply (simp add: pred_conj_def cong: if_cong)
+                  apply (wp injection_wp_E[OF refl] checkValidIPCBuffer_ArchObject_wp)
+                  apply simp
                   apply (wp | wp_once hoare_drop_imps)+
-                 apply (clarsimp simp: Collect_const_mem all_ex_eq_helper
+                 apply (simp add: Collect_const_mem all_ex_eq_helper)
+                 apply (rule_tac P="{s. cRootCap_' s = cRootCap \<and> vRootCap_' s = vRootCap
+                                        \<and> bufferAddr_' s = args ! 3
+                                        \<and> ccap_relation cp cap' \<and> isThreadCap cp
+                                        \<and> is_aligned (capTCBPtr cp) tcbBlockSizeBits
+                                        \<and> ksCurThread_' (globals s) = tcb_ptr_to_ctcb_ptr thread}"
+                          in conseqPre)
+                  apply (simp add: cong: option.case_cong)
+                  apply (vcg exspec=deriveCap_modifies exspec=checkValidIPCBuffer_modifies)
+                 apply (clarsimp simp: excaps_map_def Collect_const_mem ccHoarePost_def
+                                       numeral_eqs
                                  cong: option.case_cong)
-                 apply vcg
-                apply simp
+                 apply (frule interpret_excaps_eq[rule_format, where n=0], clarsimp)
+                 apply (frule interpret_excaps_eq[rule_format, where n=1], clarsimp)
+                 apply (frule interpret_excaps_eq[rule_format, where n=2], clarsimp)
+                 apply (clarsimp simp: mask_def[where n=4] ccap_rights_relation_def
+                                       rightsFromWord_wordFromRights capTCBPtr_eq
+                                       ptr_val_tcb_ptr_mask2[unfolded mask_def objBits_defs, simplified]
+                                       tcb_cnode_index_defs size_of_def
+                                       option_to_0_def rf_sr_ksCurThread
+                                       StrictC'_thread_state_defs mask_eq_iff_w2p word_size
+                                       from_bool_all_helper all_ex_eq_helper
+                                       ucast_ucast_mask objBits_defs)
+                 apply (subgoal_tac "args \<noteq> [] \<and> extraCaps \<noteq> []")
+                  apply (simp add: word_sle_def cap_get_tag_isCap numeral_eqs
+                                   hd_conv_nth hd_drop_conv_nth2
+                                   word_FF_is_mask split_def
+                                   thread_control_update_priority_def
+                                   thread_control_update_mcp_def
+                                   thread_control_update_space_def
+                                   thread_control_update_ipc_buffer_def)
+                  apply (auto split: option.split elim!: inl_inrE)[1]
+                  apply (fastforce+)[2]
+                apply clarsimp
+                apply (strengthen if_n_updateCapData_valid_strg)
                 apply (wp | wp_once hoare_drop_imps)+
-               apply (simp add: Collect_const_mem all_ex_eq_helper)
+               apply (clarsimp simp: Collect_const_mem all_ex_eq_helper
+                               cong: option.case_cong)
                apply vcg
               apply simp
               apply (wp | wp_once hoare_drop_imps)+
+             apply (simp add: Collect_const_mem all_ex_eq_helper)
              apply vcg
-            apply wp
-           apply (vcg exspec=getSyscallArg_modifies)
-          apply wp
-         apply (vcg exspec=getSyscallArg_modifies)
-        apply wp
-        apply simp
-       apply (vcg exspec=getSyscallArg_modifies)
-      apply wp
-     apply (vcg exspec=getSyscallArg_modifies)
-    apply wp
-   apply (vcg exspec=getSyscallArg_modifies)
-  apply (clarsimp simp: Collect_const_mem all_ex_eq_helper if_1_0_0)
+            apply simp
+            apply (wp | wp_once hoare_drop_imps)+
+           apply (wpsimp | vcg exspec=getSyscallArg_modifies)+
+  apply (clarsimp simp: Collect_const_mem all_ex_eq_helper)
   apply (rule conjI)
    apply (clarsimp simp: idButNot_def interpret_excaps_test_null
                          excaps_map_def neq_Nil_conv)
    apply (clarsimp simp: sysargs_rel_to_n word_less_nat_alt)
    apply (frule invs_mdb')
-   apply (simp add: maxPriority_def numPriorities_def)
-   apply (fold max_word_def[where 'a=8, simplified])
    apply (frule(2) tcb_at_capTCBPtr_CL)
    apply (rule conjI, fastforce)
    apply (drule interpret_excaps_eq)
@@ -3327,174 +3261,450 @@ lemma decodeTCBConfigure_ccorres:
                         tcb_cnode_index_defs size_of_def
                         option_to_0_def rf_sr_ksCurThread
                         StrictC'_thread_state_defs mask_eq_iff_w2p word_size
-                        thread_control_update_all_or
                         from_bool_all_helper)
   apply (frule(1) tcb_at_h_t_valid [OF tcb_at_invs'])
-  apply (simp add: ucast_ucast_mask exception_defs)
   apply (clarsimp simp: typ_heap_simps numeral_eqs isCap_simps valid_cap'_def capAligned_def
                         objBits_simps)
   done
 
+lemma not_isThreadCap_case:
+  "\<lbrakk>\<not>isThreadCap cap\<rbrakk> \<Longrightarrow>
+   (case cap of ThreadCap x \<Rightarrow> f x | _ \<Rightarrow> g) = g"
+  by (clarsimp simp: isThreadCap_def split: capability.splits)
+
 lemma decodeSetMCPriority_ccorres:
-  "ccorres (intr_and_se_rel \<currency> dc) (liftxf errstate id (K ()) ret__unsigned_long_')
+  "\<lbrakk>interpret_excaps extraCaps' = excaps_map extraCaps\<rbrakk> \<Longrightarrow>
+   ccorres (intr_and_se_rel \<currency> dc) (liftxf errstate id (K ()) ret__unsigned_long_')
        (invs' and (\<lambda>s. ksCurThread s = thread)
               and ct_active' and sch_act_simple
+              and (excaps_in_mem extraCaps \<circ> ctes_of)
               and (\<lambda>s. \<forall>rf \<in> zobj_refs' cp. ex_nonz_cap_to' rf s)
               and valid_cap' cp and K (isThreadCap cp)
+              and (\<lambda>s. \<forall>v \<in> set extraCaps.
+                             ex_cte_cap_wp_to' isCNodeCap (snd v) s)
+              and (\<lambda>s. \<forall>v \<in> set extraCaps.
+                             s \<turnstile>' fst v \<and> cte_at' (snd v) s)
               and sysargs_rel args buffer)
        (UNIV
             \<inter> {s. ccap_relation cp (cap_' s)}
             \<inter> {s. unat (length___unsigned_long_' s) = length args}
+            \<inter> {s. excaps_' s = extraCaps'}
             \<inter> {s. buffer_' s = option_to_ptr buffer}) []
-     (decodeSetMCPriority args cp
+     (decodeSetMCPriority args cp extraCaps
             >>= invocationCatch thread isBlocking isCall InvokeTCB)
      (Call decodeSetMCPriority_'proc)"
-  apply (cinit' lift: cap_' length___unsigned_long_' buffer_' simp: decodeSetMCPriority_def)
-   apply wpc
-    apply (simp add: throwError_bind invocationCatch_def)
-    apply (rule ccorres_from_vcg_split_throws[where P=\<top> and P'=UNIV])
-     apply vcg
-    apply (rule conseqPre, vcg)
-    apply (clarsimp simp: throwError_def return_def intr_and_se_rel_def
-                          exception_defs syscall_error_rel_def
-                          syscall_error_to_H_cases)
-   apply (rule ccorres_cond_false_seq; simp)
-   apply (rule ccorres_add_return,
-          ctac add: getSyscallArg_ccorres_foo'[where args=args and n=0 and buffer=buffer])
-     apply (simp add: invocationCatch_use_injection_handler injection_bindE[OF refl refl]
-                      bindE_assoc injection_handler_returnOk
-                 del: Collect_const)
-     apply (ctac add: ccorres_injection_handler_csum1[OF checkPrio_ccorres])
-        apply (rule_tac P="newMcp \<le> ucast (max_word :: priority)"
-               in ccorres_cross_over_guard_no_st)
-        apply (simp add: ccorres_invocationCatch_Inr performInvocation_def)
-        apply (ctac add: setThreadState_ccorres)
-          apply csymbr
-          apply csymbr
-          apply csymbr
-          apply csymbr
-          apply (ctac (no_vcg) add: invokeTCB_ThreadControl_ccorres)
-            apply simp
-            apply (rule ccorres_alternative2)
-            apply (rule ccorres_return_CE, simp+)[1]
-           apply (rule ccorres_return_C_errorE, simp+)[1]
-          apply wp
+  supply Collect_const[simp del]
+  supply dc_simp[simp del]
+  apply (cinit' lift: cap_' length___unsigned_long_' excaps_' buffer_' simp: decodeSetMCPriority_def)
+   apply (simp cong: StateSpace.state.fold_congs globals.fold_congs)
+   apply (rule ccorres_rhs_assoc2)
+   apply (rule_tac xf'=ret__int_' and R'=UNIV and R=\<top> and
+                   val="from_bool (length args = 0 \<or> length extraCaps = 0)" in
+                   ccorres_symb_exec_r_known_rv)
+      apply vcg
+      apply (force simp: interpret_excaps_test_null excaps_map_def from_bool_def unat_eq_0
+                   split: bool.splits)
+     apply ceqv
+    apply clarsimp
+    apply wpc
+     (* Case args = [] *)
+     apply (rule ccorres_cond_true_seq)
+     apply (clarsimp simp: throwError_bind invocationCatch_def)
+     apply (rule ccorres_rhs_assoc)
+     apply (ccorres_rewrite)
+     apply (rule syscall_error_throwError_ccorres_n)
+     apply (simp add: syscall_error_to_H_cases)
+    (* Case args is Cons *)
+    apply wpc
+     (* Sub-case extraCaps = [] *)
+     apply (rule ccorres_cond_true_seq)
+     apply (clarsimp simp: throwError_bind invocationCatch_def)
+     apply (rule ccorres_rhs_assoc)
+     apply (ccorres_rewrite)
+     apply (rule syscall_error_throwError_ccorres_n)
+     apply (simp add: syscall_error_to_H_cases)
+    (* Main case where args and extraCaps are both Cons *)
+    apply (rule ccorres_cond_false_seq)
+    apply (simp add: split_def)
+    apply (rule ccorres_add_return,
+           ctac add: getSyscallArg_ccorres_foo'[where args=args and n=0 and buffer=buffer])
+      apply (rule getSlotCap_ccorres_fudge_n[where vals=extraCaps and n=0])
+      apply (rule ccorres_move_c_guard_cte)
+      apply ctac
+        apply csymbr
+        apply (simp add: cap_get_tag_isCap cong: call_ignore_cong)
+        apply (rule ccorres_assert2)
+        apply (rule ccorres_Cond_rhs_Seq)
+         apply (rule ccorres_rhs_assoc)
+         apply ccorres_rewrite
+         apply (clarsimp simp: not_isThreadCap_case throwError_bind invocationCatch_def
+                         simp del: id_simps)
+         apply (rule syscall_error_throwError_ccorres_n)
+         apply (simp add: syscall_error_to_H_cases)
+        apply (clarsimp simp: isCap_simps)
+        apply csymbr
+        apply csymbr
+        (* Pre-conditions need to depend on the inner value of the thread cap *)
+        apply (rule ccorres_inst[where P="Q (capTCBPtr (fst (extraCaps ! 0)))" and
+                                       P'="Q' (capTCBPtr (fst (extraCaps ! 0)))" for Q Q'])
+        apply (clarsimp simp: capTCBPtr_eq isCap_simps invocationCatch_use_injection_handler
+                              injection_bindE[OF refl refl] bindE_assoc injection_handler_returnOk)
+        apply (ctac add: ccorres_injection_handler_csum1[OF checkPrio_ccorres])
+           apply (rule_tac P="hd args \<le> ucast (max_word :: priority)"
+                           in ccorres_cross_over_guard_no_st)
+           apply (simp add: ccorres_invocationCatch_Inr performInvocation_def)
+           apply ccorres_rewrite
+           apply (ctac add: setThreadState_ccorres)
+             apply (simp add: invocationCatch_def)
+             apply ccorres_rewrite
+             apply csymbr
+             apply csymbr
+             apply csymbr
+             apply csymbr
+             apply (ctac (no_vcg) add: invokeTCB_ThreadControl_ccorres)
+               (* HACK: delete rules from the simpset to avoid the RVRs getting out of sync *)
+               apply (clarsimp simp del: intr_and_se_rel_simps comp_apply dc_simp)
+               apply (rule ccorres_alternative2)
+               apply (rule ccorres_return_CE; simp)
+              apply (rule ccorres_return_C_errorE; simp)
+             apply wp
+            apply (wpsimp wp: sts_invs_minor')
+           apply simp
+           apply (vcg exspec=setThreadState_modifies)
+          apply simp
+          apply (rename_tac err_c)
+          apply (rule_tac P'="{s. err_c = errstate s}" in ccorres_from_vcg_split_throws)
+           apply vcg
+          apply (rule conseqPre, vcg)
+          apply (clarsimp simp: throwError_def return_def intr_and_se_rel_def syscall_error_rel_def)
          apply simp
-         apply (wp sts_invs_minor')
-        apply (vcg exspec=setThreadState_modifies)
-       apply simp
-       apply (rename_tac err_c)
-       apply (rule_tac P'="{s. err_c = errstate s}" in ccorres_from_vcg_split_throws)
+         apply (rule injection_handler_wp)
+         apply (rule checkPrio_wp[simplified validE_R_def])
         apply vcg
-       apply (rule conseqPre, vcg)
-       apply (clarsimp simp: throwError_def return_def intr_and_se_rel_def syscall_error_rel_def)
-      apply simp
-      apply (rule injection_handler_wp)
-      apply (rule checkPrio_wp[simplified validE_R_def])
-     apply (simp; vcg)
-    apply wp
-   apply (simp; vcg)
-  apply (clarsimp simp: Collect_const_mem intr_and_se_rel_def
-                        syscall_error_rel_def syscall_error_to_H_cases
-                        exception_defs)
+       apply (wp | simp | wpc | wp_once hoare_drop_imps)+
+      apply vcg
+     apply wp
+    apply (vcg exspec=getSyscallArg_modifies)
+   apply (clarsimp simp: EXCEPTION_SYSCALL_ERROR_def EXCEPTION_NONE_def)
+   apply vcg
+  apply clarsimp
   apply (rule conjI)
    apply (clarsimp simp: ct_in_state'_def pred_tcb_at'
                          valid_cap'_def isCap_simps)
    apply (rule conjI, clarsimp simp: sysargs_rel_n_def n_msgRegisters_def)
    apply (clarsimp simp: maxPriority_def numPriorities_def)
    apply (fold max_word_def[where 'a=8, simplified])
-   apply (frule mcpriority_tcb_at'_prio_bounded, simp)
-   apply (auto simp: valid_tcb_state'_def le_ucast_ucast_le
-              elim!: obj_at'_weakenE pred_tcb'_weakenE
-              dest!: st_tcb_at_idle_thread')[1]
-  apply (simp add: StrictC'_thread_state_defs mask_eq_iff_w2p word_size
-                   option_to_0_def)
+   apply (rule conjI, clarsimp)
+    apply (frule mcpriority_tcb_at'_prio_bounded, simp)
+    apply (auto simp: valid_tcb_state'_def le_ucast_ucast_le
+                elim!: obj_at'_weakenE pred_tcb'_weakenE
+                dest!: st_tcb_at_idle_thread')[1]
+   apply (clarsimp simp: interpret_excaps_eq excaps_map_def)
+  apply (simp add: StrictC'_thread_state_defs mask_eq_iff_w2p word_size option_to_0_def)
   apply (frule rf_sr_ksCurThread)
   apply (simp only: cap_get_tag_isCap[symmetric], drule(1) cap_get_tag_to_H)
-  apply (clarsimp simp: valid_cap'_def capAligned_def)
+  apply (clarsimp simp: valid_cap'_def capAligned_def interpret_excaps_eq excaps_map_def)
   apply (intro conjI impI allI)
-       apply (clarsimp simp: unat_eq_0 le_max_word_ucast_id)+
+   apply (clarsimp simp: unat_eq_0 le_max_word_ucast_id cap_get_tag_isCap_unfolded_H_cap isCap_simps)+
   done
 
 lemma decodeSetPriority_ccorres:
-  "ccorres (intr_and_se_rel \<currency> dc) (liftxf errstate id (K ()) ret__unsigned_long_')
+  "\<lbrakk>interpret_excaps extraCaps' = excaps_map extraCaps\<rbrakk> \<Longrightarrow>
+   ccorres (intr_and_se_rel \<currency> dc) (liftxf errstate id (K ()) ret__unsigned_long_')
        (invs' and (\<lambda>s. ksCurThread s = thread)
               and ct_active' and sch_act_simple
+              and (excaps_in_mem extraCaps \<circ> ctes_of)
               and (\<lambda>s. \<forall>rf \<in> zobj_refs' cp. ex_nonz_cap_to' rf s)
               and valid_cap' cp and K (isThreadCap cp)
+              and (\<lambda>s. \<forall>v \<in> set extraCaps.
+                             ex_cte_cap_wp_to' isCNodeCap (snd v) s)
+              and (\<lambda>s. \<forall>v \<in> set extraCaps.
+                             s \<turnstile>' fst v \<and> cte_at' (snd v) s)
               and sysargs_rel args buffer)
        (UNIV
             \<inter> {s. ccap_relation cp (cap_' s)}
             \<inter> {s. unat (length___unsigned_long_' s) = length args}
+            \<inter> {s. excaps_' s = extraCaps'}
             \<inter> {s. buffer_' s = option_to_ptr buffer}) []
-     (decodeSetPriority args cp
+     (decodeSetPriority args cp extraCaps
             >>= invocationCatch thread isBlocking isCall InvokeTCB)
      (Call decodeSetPriority_'proc)"
-  apply (cinit' lift: cap_' length___unsigned_long_' buffer_' simp: decodeSetPriority_def)
-   apply wpc
-    apply (simp add: throwError_bind invocationCatch_def)
-    apply (rule ccorres_from_vcg_split_throws[where P=\<top> and P'=UNIV])
-     apply vcg
-    apply (rule conseqPre, vcg)
-    apply (clarsimp simp: throwError_def return_def intr_and_se_rel_def
-                          exception_defs syscall_error_rel_def
-                          syscall_error_to_H_cases)
-   apply (rule ccorres_cond_false_seq; simp)
-   apply (rule ccorres_add_return,
-          ctac add: getSyscallArg_ccorres_foo'[where args=args and n=0 and buffer=buffer])
-     apply (simp add: invocationCatch_use_injection_handler injection_bindE[OF refl refl]
-                      bindE_assoc injection_handler_returnOk
-                 del: Collect_const)
-     apply (ctac add: ccorres_injection_handler_csum1[OF checkPrio_ccorres])
-        apply (rule_tac P="newPrio \<le> ucast (max_word :: priority)"
-               in ccorres_cross_over_guard_no_st)
-        apply (simp add: ccorres_invocationCatch_Inr performInvocation_def)
-        apply (ctac add: setThreadState_ccorres)
-          apply csymbr
-          apply csymbr
-          apply csymbr
-          apply csymbr
-          apply (ctac (no_vcg) add: invokeTCB_ThreadControl_ccorres)
-            apply simp
-            apply (rule ccorres_alternative2)
-            apply (rule ccorres_return_CE, simp+)[1]
-           apply (rule ccorres_return_C_errorE, simp+)[1]
-          apply wp
+  supply Collect_const[simp del] dc_simp[simp del]
+  apply (cinit' lift: cap_' length___unsigned_long_' excaps_' buffer_' simp: decodeSetPriority_def)
+     apply (simp cong: StateSpace.state.fold_congs globals.fold_congs)
+   apply (rule ccorres_rhs_assoc2)
+   apply (rule_tac xf'=ret__int_' and R'=UNIV and R=\<top> and
+                   val="from_bool (length args = 0 \<or> length extraCaps = 0)" in
+                   ccorres_symb_exec_r_known_rv)
+      apply vcg
+      apply (force simp: interpret_excaps_test_null excaps_map_def from_bool_def unat_eq_0
+                   split: bool.splits)
+     apply ceqv
+    apply clarsimp
+    apply wpc
+     (* Case args = [] *)
+     apply (rule ccorres_cond_true_seq)
+     apply (clarsimp simp: throwError_bind invocationCatch_def)
+     apply (rule ccorres_rhs_assoc)
+     apply (ccorres_rewrite)
+     apply (rule syscall_error_throwError_ccorres_n)
+     apply (simp add: syscall_error_to_H_cases)
+    (* Case args is Cons *)
+    apply wpc
+     (* Sub-case extraCaps = [] *)
+     apply (rule ccorres_cond_true_seq)
+     apply (clarsimp simp: throwError_bind invocationCatch_def)
+     apply (rule ccorres_rhs_assoc)
+     apply (ccorres_rewrite)
+     apply (rule syscall_error_throwError_ccorres_n)
+     apply (simp add: syscall_error_to_H_cases)
+    (* Main case where args and extraCaps are both Cons *)
+    apply (rule ccorres_cond_false_seq)
+    apply (simp add: split_def)
+    apply (rule ccorres_add_return,
+           ctac add: getSyscallArg_ccorres_foo'[where args=args and n=0 and buffer=buffer])
+      apply (rule getSlotCap_ccorres_fudge_n[where vals=extraCaps and n=0])
+      apply (rule ccorres_move_c_guard_cte)
+      apply ctac
+        apply csymbr
+        apply (simp add: cap_get_tag_isCap cong: call_ignore_cong)
+        apply (rule ccorres_assert2)
+        apply (rule ccorres_Cond_rhs_Seq)
+         apply (rule ccorres_rhs_assoc)
+         apply ccorres_rewrite
+         apply (clarsimp simp: not_isThreadCap_case throwError_bind invocationCatch_def
+                         simp del: id_simps)
+         apply (rule syscall_error_throwError_ccorres_n)
+         apply (simp add: syscall_error_to_H_cases)
+        apply (clarsimp simp: isCap_simps)
+        apply csymbr
+        apply csymbr
+        (* Pre-conditions need to depend on the inner value of the thread cap *)
+        apply (rule ccorres_inst[where P="Q (capTCBPtr (fst (extraCaps ! 0)))" and
+                                       P'="Q' (capTCBPtr (fst (extraCaps ! 0)))" for Q Q'])
+        apply (clarsimp simp: capTCBPtr_eq isCap_simps invocationCatch_use_injection_handler
+                              injection_bindE[OF refl refl] bindE_assoc injection_handler_returnOk)
+        apply (ctac add: ccorres_injection_handler_csum1[OF checkPrio_ccorres])
+           apply (rule_tac P="hd args \<le> ucast (max_word :: priority)"
+                           in ccorres_cross_over_guard_no_st)
+           apply (simp add: ccorres_invocationCatch_Inr performInvocation_def)
+           apply ccorres_rewrite
+           apply (ctac add: setThreadState_ccorres)
+             apply (simp add: invocationCatch_def)
+             apply ccorres_rewrite
+             apply csymbr
+             apply csymbr
+             apply csymbr
+             apply csymbr
+             apply (ctac (no_vcg) add: invokeTCB_ThreadControl_ccorres)
+               (* HACK: delete rules from the simpset to avoid the RVRs getting out of sync *)
+               apply (clarsimp simp del: intr_and_se_rel_simps comp_apply dc_simp)
+               apply (rule ccorres_alternative2)
+               apply (rule ccorres_return_CE; simp)
+              apply (rule ccorres_return_C_errorE; simp)
+             apply wp
+            apply (wpsimp wp: sts_invs_minor')
+           apply simp
+           apply (vcg exspec=setThreadState_modifies)
+          apply simp
+          apply (rename_tac err_c)
+          apply (rule_tac P'="{s. err_c = errstate s}" in ccorres_from_vcg_split_throws)
+           apply vcg
+          apply (rule conseqPre, vcg)
+          apply (clarsimp simp: throwError_def return_def intr_and_se_rel_def syscall_error_rel_def)
          apply simp
-         apply (wp sts_invs_minor')
-        apply (vcg exspec=setThreadState_modifies)
-       apply simp
-       apply (rename_tac err_c)
-       apply (rule_tac P'="{s. err_c = errstate s}" in ccorres_from_vcg_split_throws)
+         apply (rule injection_handler_wp)
+         apply (rule checkPrio_wp[simplified validE_R_def])
         apply vcg
-       apply (rule conseqPre, vcg)
-       apply (clarsimp simp: throwError_def return_def intr_and_se_rel_def syscall_error_rel_def)
-      apply simp
-      apply (rule injection_handler_wp)
-      apply (rule checkPrio_wp[simplified validE_R_def])
-     apply (simp; vcg)
-    apply wp
-   apply (simp; vcg)
-  apply (clarsimp simp: Collect_const_mem intr_and_se_rel_def
-                        syscall_error_rel_def syscall_error_to_H_cases
-                        exception_defs)
+       apply (wp | simp | wpc | wp_once hoare_drop_imps)+
+      apply vcg
+     apply wp
+    apply (vcg exspec=getSyscallArg_modifies)
+   apply (clarsimp simp: EXCEPTION_SYSCALL_ERROR_def EXCEPTION_NONE_def)
+   apply vcg
+  apply clarsimp
   apply (rule conjI)
    apply (clarsimp simp: ct_in_state'_def pred_tcb_at'
                          valid_cap'_def isCap_simps)
    apply (rule conjI, clarsimp simp: sysargs_rel_n_def n_msgRegisters_def)
    apply (clarsimp simp: maxPriority_def numPriorities_def)
    apply (fold max_word_def[where 'a=8, simplified])
-   apply (frule mcpriority_tcb_at'_prio_bounded, simp)
-   apply (auto simp: valid_tcb_state'_def le_ucast_ucast_le
-              elim!: obj_at'_weakenE pred_tcb'_weakenE
-              dest!: st_tcb_at_idle_thread')[1]
-  apply (simp add: StrictC'_thread_state_defs mask_eq_iff_w2p word_size
-                   option_to_0_def)
+   apply (rule conjI, clarsimp)
+    apply (frule mcpriority_tcb_at'_prio_bounded, simp)
+    apply (auto simp: valid_tcb_state'_def le_ucast_ucast_le
+                elim!: obj_at'_weakenE pred_tcb'_weakenE
+                dest!: st_tcb_at_idle_thread')[1]
+   apply (clarsimp simp: interpret_excaps_eq excaps_map_def)
+  apply (simp add: StrictC'_thread_state_defs mask_eq_iff_w2p word_size option_to_0_def)
   apply (frule rf_sr_ksCurThread)
   apply (simp only: cap_get_tag_isCap[symmetric], drule(1) cap_get_tag_to_H)
-  apply (clarsimp simp: valid_cap'_def capAligned_def)
+  apply (clarsimp simp: valid_cap'_def capAligned_def interpret_excaps_eq excaps_map_def)
   apply (intro conjI impI allI)
-       apply (clarsimp simp: unat_eq_0 le_max_word_ucast_id)+
+   apply (clarsimp simp: unat_eq_0 le_max_word_ucast_id cap_get_tag_isCap_unfolded_H_cap isCap_simps)+
+  done
+
+lemma ucast_le_8_32_equiv:
+  "x \<le> UCAST (8 \<rightarrow> 32) max_word \<Longrightarrow>
+  (UCAST (32 \<rightarrow> 8) x \<le> y) = (x \<le> UCAST (8 \<rightarrow> 32) y)"
+  apply (rule iffI)
+   apply (word_bitwise; simp)
+  apply (simp add: le_ucast_ucast_le)
+  done
+
+lemma mcpriority_tcb_at'_le_ucast:
+  "pred_tcb_at' itcbMCP (\<lambda>mcp. x \<le> UCAST(8 \<rightarrow> 32) mcp) v s \<Longrightarrow>
+   pred_tcb_at' itcbMCP (\<lambda>mcp. UCAST(32 \<rightarrow> 8) x \<le> mcp) v s"
+  apply (clarsimp simp: ucast_le_8_32_equiv mcpriority_tcb_at'_prio_bounded)
+  done
+
+lemma decodeSetSchedParams_ccorres:
+  "\<lbrakk>interpret_excaps extraCaps' = excaps_map extraCaps\<rbrakk> \<Longrightarrow>
+   ccorres (intr_and_se_rel \<currency> dc) (liftxf errstate id (K ()) ret__unsigned_long_')
+       (invs' and (\<lambda>s. ksCurThread s = thread)
+              and ct_active' and sch_act_simple
+              and (excaps_in_mem extraCaps \<circ> ctes_of)
+              and (\<lambda>s. \<forall>rf \<in> zobj_refs' cp. ex_nonz_cap_to' rf s)
+              and valid_cap' cp and K (isThreadCap cp)
+              and (\<lambda>s. \<forall>v \<in> set extraCaps.
+                             ex_cte_cap_wp_to' isCNodeCap (snd v) s)
+              and (\<lambda>s. \<forall>v \<in> set extraCaps.
+                             s \<turnstile>' fst v \<and> cte_at' (snd v) s)
+              and sysargs_rel args buffer)
+       (UNIV
+            \<inter> {s. ccap_relation cp (cap_' s)}
+            \<inter> {s. unat (length___unsigned_long_' s) = length args}
+            \<inter> {s. excaps_' s = extraCaps'}
+            \<inter> {s. buffer_' s = option_to_ptr buffer}) []
+     (decodeSetSchedParams args cp extraCaps
+            >>= invocationCatch thread isBlocking isCall InvokeTCB)
+     (Call decodeSetSchedParams_'proc)"
+  supply Collect_const[simp del] dc_simp[simp del]
+  apply (cinit' lift: cap_' length___unsigned_long_' excaps_' buffer_' simp: decodeSetSchedParams_def)
+   apply (simp cong: StateSpace.state.fold_congs globals.fold_congs)
+   apply (rule ccorres_rhs_assoc2)
+   apply (rule_tac xf'=ret__int_' and R'=UNIV and R=\<top> and
+                   val="from_bool (length args < 2 \<or> length extraCaps = 0)" in
+                   ccorres_symb_exec_r_known_rv)
+      apply vcg
+      apply (auto simp: interpret_excaps_test_null excaps_map_def from_bool_def unat_eq_0
+                  split: bool.splits)[1]
+       apply (unat_arith+)[2]
+     apply ceqv
+    apply clarsimp
+    apply (wpc,
+           rule ccorres_cond_true_seq,
+           clarsimp simp: throwError_bind invocationCatch_def,
+           rule ccorres_rhs_assoc,
+           ccorres_rewrite,
+           fastforce intro: syscall_error_throwError_ccorres_n simp: syscall_error_to_H_cases)+
+    (* Main case where args and extraCaps are both well-formed *)
+    apply (rule ccorres_cond_false_seq)
+    apply (simp add: split_def)
+    apply (rule ccorres_add_return,
+           ctac add: getSyscallArg_ccorres_foo'[where args=args and n=0 and buffer=buffer])
+      apply (rule ccorres_add_return,
+             ctac add: getSyscallArg_ccorres_foo'[where args=args and n=1 and buffer=buffer])
+        apply (rule getSlotCap_ccorres_fudge_n[where vals=extraCaps and n=0])
+        apply (rule ccorres_move_c_guard_cte)
+        apply ctac
+          apply csymbr
+          apply (simp add: cap_get_tag_isCap cong: call_ignore_cong)
+          apply (rule ccorres_assert2)
+          apply (rule ccorres_Cond_rhs_Seq)
+           apply (rule ccorres_rhs_assoc)
+           apply ccorres_rewrite
+           apply (clarsimp simp: not_isThreadCap_case throwError_bind invocationCatch_def
+                           simp del: id_simps)
+           apply (rule syscall_error_throwError_ccorres_n)
+           apply (simp add: syscall_error_to_H_cases)
+          apply (clarsimp simp: isCap_simps)
+          apply csymbr
+          apply csymbr
+          (* Pre-conditions need to depend on the inner value of the thread cap *)
+          apply (rule ccorres_inst[where P="Q (capTCBPtr (fst (extraCaps ! 0)))" and
+                                         P'="Q' (capTCBPtr (fst (extraCaps ! 0)))" for Q Q'])
+          apply (clarsimp simp: capTCBPtr_eq isCap_simps invocationCatch_use_injection_handler
+                                injection_bindE[OF refl refl] bindE_assoc injection_handler_returnOk)
+          apply (ctac add: ccorres_injection_handler_csum1[OF checkPrio_ccorres])
+             apply (rule_tac P="args ! 0 \<le> ucast (max_word :: priority)"
+                             in ccorres_cross_over_guard_no_st)
+             apply (simp add: ccorres_invocationCatch_Inr performInvocation_def)
+             apply ccorres_rewrite
+             apply (clarsimp simp: capTCBPtr_eq isCap_simps invocationCatch_use_injection_handler
+                                   injection_bindE[OF refl refl] bindE_assoc injection_handler_returnOk)
+             apply (ctac add: ccorres_injection_handler_csum1[OF checkPrio_ccorres])
+                apply (rule_tac P="args ! 1 \<le> ucast (max_word :: priority)"
+                                in ccorres_cross_over_guard_no_st)
+                apply (simp add: ccorres_invocationCatch_Inr performInvocation_def)
+                apply ccorres_rewrite
+                apply (ctac add: setThreadState_ccorres)
+                  apply (simp add: invocationCatch_def)
+                  apply ccorres_rewrite
+                  apply csymbr
+                  apply csymbr
+                  apply csymbr
+                  apply csymbr
+                  apply (ctac (no_vcg) add: invokeTCB_ThreadControl_ccorres)
+                    (* HACK: delete rules from the simpset to avoid the RVRs getting out of sync *)
+                    apply (clarsimp simp del: intr_and_se_rel_simps comp_apply dc_simp)
+                    apply (rule ccorres_alternative2)
+                    apply (rule ccorres_return_CE; simp)
+                   apply (rule ccorres_return_C_errorE; simp)
+                  apply wp
+                 apply (wpsimp wp: sts_invs_minor')
+                apply simp
+                apply (vcg exspec=setThreadState_modifies)
+               apply simp
+               apply (rename_tac err_c)
+               apply (rule_tac P'="{s. err_c = errstate s}" in ccorres_from_vcg_split_throws)
+                apply vcg
+               apply (rule conseqPre, vcg)
+               apply (clarsimp simp: throwError_def return_def intr_and_se_rel_def syscall_error_rel_def)
+              apply simp
+              apply (rule injection_handler_wp)
+              apply (rule checkPrio_wp[simplified validE_R_def])
+             apply vcg
+            apply clarsimp
+            apply ccorres_rewrite
+            apply (rule ccorres_return_C_errorE; simp)
+           apply simp
+           apply (rule injection_handler_wp)
+           apply (rule checkPrio_wp[simplified validE_R_def])
+          apply vcg
+         apply (wp | simp | wpc | wp_once hoare_drop_imps)+
+        apply vcg
+       apply simp
+       apply (rule return_wp)
+      apply (vcg exspec=getSyscallArg_modifies)
+     apply simp
+     apply (rule return_wp)
+    apply simp
+    apply (vcg exspec=getSyscallArg_modifies)
+   apply simp
+   apply (vcg exspec=getSyscallArg_modifies)
+  apply clarsimp
+  apply (rule conjI)
+   apply (clarsimp simp: ct_in_state'_def pred_tcb_at'
+      valid_cap'_def isCap_simps)
+   apply (rule conjI; clarsimp simp: sysargs_rel_to_n n_msgRegisters_def)
+   apply (clarsimp simp: maxPriority_def numPriorities_def)
+   apply (fold max_word_def[where 'a=8, simplified])
+   apply (rule conjI, clarsimp)
+    apply (insert mcpriority_tcb_at'_prio_bounded[where prio="args ! 0"])
+    apply (insert mcpriority_tcb_at'_prio_bounded[where prio="args ! 1"])
+    apply (auto simp: valid_tcb_state'_def mcpriority_tcb_at'_le_ucast
+                elim!: obj_at'_weakenE pred_tcb'_weakenE
+                dest!: st_tcb_at_idle_thread')[1]
+   apply (clarsimp simp: interpret_excaps_eq excaps_map_def)
+  apply (simp add: StrictC'_thread_state_defs mask_eq_iff_w2p word_size option_to_0_def)
+  apply (frule rf_sr_ksCurThread)
+  apply (simp only: cap_get_tag_isCap[symmetric], drule(1) cap_get_tag_to_H)
+  apply (clarsimp simp: valid_cap'_def capAligned_def interpret_excaps_eq excaps_map_def)
+  apply (intro conjI impI allI)
+                      apply (clarsimp simp: unat_eq_0 le_max_word_ucast_id
+                                            thread_control_update_mcp_def thread_control_update_priority_def
+                                            cap_get_tag_isCap_unfolded_H_cap isCap_simps
+                                            interpret_excaps_eq excaps_map_def)+
   done
 
 lemma decodeSetIPCBuffer_ccorres:
@@ -3534,6 +3744,7 @@ lemma decodeSetIPCBuffer_ccorres:
    apply csymbr
    apply (rule ccorres_cond_false_seq)
    apply csymbr
+   apply (simp del: Collect_const)
    apply (simp add: interpret_excaps_test_null excaps_map_Nil if_1_0_0
                del: Collect_const)
    apply wpc
@@ -4381,6 +4592,12 @@ lemma decodeTCBInvocation_ccorres:
    apply (rule ccorres_Cond_rhs)
     apply simp
     apply (rule ccorres_add_returnOk, ctac(no_vcg) add: decodeSetMCPriority_ccorres [where buffer=buffer])
+      apply (rule ccorres_return_CE, simp+)[1]
+     apply (rule ccorres_return_C_errorE, simp+)[1]
+    apply wp
+   apply (rule ccorres_Cond_rhs)
+    apply simp
+    apply (rule ccorres_add_returnOk, ctac(no_vcg) add: decodeSetSchedParams_ccorres [where buffer=buffer])
       apply (rule ccorres_return_CE, simp+)[1]
      apply (rule ccorres_return_C_errorE, simp+)[1]
     apply wp
