proof/invariant-abstract/ARM/ArchEmptyFail_AI.thy
@@ -43,7 +43,8 @@ crunch (empty_fail) empty_fail[wp, EmptyFail_AI_assms]: handle_fault
          bool.splits list.splits thread_state.splits split_def catch_def sum.splits
          Let_def wp: zipWithM_x_empty_fail)
 
-crunch (empty_fail) empty_fail[wp]: decode_tcb_configure, decode_bind_notification, decode_unbind_notification
+crunch (empty_fail) empty_fail[wp]: decode_tcb_configure, decode_bind_notification, decode_unbind_notification,
+  decode_set_priority, decode_set_mcpriority, decode_set_sched_params
   (simp: cap.splits arch_cap.splits split_def)
 
 lemma decode_tcb_invocation_empty_fail[wp]:
