proof/invariant-abstract/X64/ArchBCorres2_AI.thy
@@ -101,7 +101,7 @@ lemma decode_cnode_invocation[wp]: "bcorres (decode_cnode_invocation a b c d) (d
   apply (wp | wpc | simp add: split_def | intro impI conjI)+
   done
 
-crunch (bcorres)bcorres[wp]: decode_set_ipc_buffer,decode_set_space,decode_set_priority,decode_set_mcpriority,decode_bind_notification,decode_unbind_notification truncate_state
+crunch (bcorres)bcorres[wp]: decode_set_ipc_buffer,decode_set_space,decode_set_priority,decode_set_mcpriority,decode_set_sched_params,decode_bind_notification,decode_unbind_notification truncate_state
 
 lemma decode_tcb_configure_bcorres[wp]: "bcorres (decode_tcb_configure b (cap.ThreadCap c) d e)
      (decode_tcb_configure b (cap.ThreadCap c) d e)"
