proof/refine/ARM_HYP/Orphanage.thy
@@ -2068,7 +2068,7 @@ lemma tc_no_orphans:
     K (case_option True (swp is_aligned msg_align_bits o fst) g) and
     K (case g of None \<Rightarrow> True | Some x \<Rightarrow> (case_option True (isArchObjectCap \<circ> fst) \<circ> snd) x) and
     K (valid_option_prio d \<and> valid_option_prio mcp) \<rbrace>
-      invokeTCB (tcbinvocation.ThreadControl a sl b' d mcp e' f' g)
+      invokeTCB (tcbinvocation.ThreadControl a sl b' mcp d e' f' g)
    \<lbrace> \<lambda>rv s. no_orphans s \<rbrace>"
   apply (rule hoare_gen_asm)
   apply (rule hoare_gen_asm)
@@ -2080,13 +2080,13 @@ lemma tc_no_orphans:
     apply ((wp case_option_wp threadSet_no_orphans threadSet_invs_trivial
                threadSet_cap_to' hoare_vcg_all_lift static_imp_wp | clarsimp simp: inQ_def)+)[2]
   apply (rule hoare_walk_assmsE)
-    apply (clarsimp simp: pred_conj_def option.splits[where P="\<lambda>x. x s" for s])
+    apply (cases mcp; clarsimp simp: pred_conj_def option.splits[where P="\<lambda>x. x s" for s])
     apply ((wp case_option_wp threadSet_no_orphans threadSet_invs_trivial setMCPriority_invs'
               typ_at_lifts[OF setMCPriority_typ_at']
-               threadSet_cap_to' hoare_vcg_all_lift static_imp_wp | clarsimp simp: inQ_def)+)[2]
+               threadSet_cap_to' hoare_vcg_all_lift static_imp_wp | clarsimp simp: inQ_def)+)[3]
   apply (rule hoare_walk_assmsE)
-    apply (clarsimp simp: pred_conj_def option.splits[where P="\<lambda>x. x s" for s])
-    apply ((wp case_option_wp hoare_vcg_all_lift static_imp_wp setP_invs' | clarsimp)+)[2]
+    apply (cases d; clarsimp simp: pred_conj_def option.splits[where P="\<lambda>x. x s" for s])
+    apply ((wp case_option_wp hoare_vcg_all_lift static_imp_wp setP_invs' | clarsimp)+)[3]
    apply (rule hoare_pre)
     apply ((simp only: simp_thms cong: conj_cong
           | wp cteDelete_deletes cteDelete_invs' cteDelete_sch_act_simple
