proof/refine/X64/Orphanage.thy
@@ -2065,13 +2065,13 @@ lemma tc_no_orphans:
     apply ((wp case_option_wp threadSet_no_orphans threadSet_invs_trivial
                threadSet_cap_to' hoare_vcg_all_lift static_imp_wp | clarsimp simp: inQ_def)+)[2]
   apply (rule hoare_walk_assmsE)
-    apply (clarsimp simp: pred_conj_def option.splits[where P="\<lambda>x. x s" for s])
+    apply (cases mcp; clarsimp simp: pred_conj_def option.splits[where P="\<lambda>x. x s" for s])
     apply ((wp case_option_wp threadSet_no_orphans threadSet_invs_trivial setMCPriority_invs'
               typ_at_lifts[OF setMCPriority_typ_at']
-               threadSet_cap_to' hoare_vcg_all_lift static_imp_wp | clarsimp simp: inQ_def)+)[2]
+               threadSet_cap_to' hoare_vcg_all_lift static_imp_wp | clarsimp simp: inQ_def)+)[3]
   apply (rule hoare_walk_assmsE)
-    apply (clarsimp simp: pred_conj_def option.splits[where P="\<lambda>x. x s" for s])
-    apply ((wp case_option_wp hoare_vcg_all_lift static_imp_wp setP_invs' | clarsimp)+)[2]
+    apply (cases d; clarsimp simp: pred_conj_def option.splits[where P="\<lambda>x. x s" for s])
+     apply ((wp case_option_wp hoare_vcg_all_lift static_imp_wp setP_invs' | clarsimp)+)[3]
   apply (rule hoare_pre)
    apply (simp only: simp_thms cong: conj_cong
           | wp cteDelete_deletes cteDelete_invs' cteDelete_sch_act_simple
