spec/abstract/Tcb_A.thy
@@ -160,9 +160,9 @@ where
    = doE
     liftE $ option_update_thread target (tcb_fault_handler_update o K) faultep;
     liftE $  case mcp of None \<Rightarrow> return()
-     | Some newmcp \<Rightarrow> set_mcpriority target newmcp;
+     | Some (newmcp, _) \<Rightarrow> set_mcpriority target newmcp;
     liftE $ case priority of None \<Rightarrow> return()
-     | Some prio \<Rightarrow> do_extended_op (set_priority target prio);
+     | Some (prio, _) \<Rightarrow> do_extended_op (set_priority target prio);
     (case croot of None \<Rightarrow> returnOk ()
      | Some (new_cap, src_slot) \<Rightarrow> doE
       cap_delete (target, tcb_cnode_index 0);
